fixes

src/MutableMap/MutableMapFeasability.dfy
@@ -1,7 +1,7 @@
 include "MutableMap.dfy"
 
 module {:options "/functionSyntax:4"} MutableMapFeasability refines MutableMap {
-  class MutableMap<K(==),V> ... {
+  class MutableMap<K(==),V(==)> ... {
     var m: map<K,V>
 
     function content(): map<K, V> {
@@ -18,14 +18,30 @@ module {:options "/functionSyntax:4"} MutableMapFeasability refines MutableMap {
       m := m[k := v];
     }
 
-    function Keys(): (keys: set<K>)
+    function Keys(): set<K>
     {
       m.Keys
     }
 
-    function Values(): (values: set<V>)
+    function Values(): set<V>
     {
       m.Values
+    }
+
+    function Items(): set<(K,V)>
+    {
+      var items := set k | k in m.Keys :: (k, m[k]);
+      assert items == m.Items by {
+        forall k | k in m.Keys ensures (k, m[k]) in m.Items {
+          assert (k, m[k]) in m.Items;
+        }
+        assert items <= m.Items;
+        forall x | x in m.Items ensures x in items {
+          assert (x.0, m[x.0]) in items;
+        }
+        assert m.Items <= items;
+      }
+      items
     }
 
     function Find(k: K): (v: V)
